spec+proofs: cleanup for capDL-related proofs
Clean up style and content for capDL-related changes.

Co-authored-by: Corey Lewis <corey.lewis@proofcraft.systems>
Signed-off-by: Gerwin Klein <gerwin.klein@proofcraft.systems>

spec/abstract/ARM/ArchVMAttributes_A.thy
@@ -11,42 +11,39 @@ imports
   ExecSpec.MachineExports
 begin
 
-context Arch begin global_naming ARM_A
+context Arch begin arch_global_naming (A)
 
 (* Union of attributes and non-seL4 rights that the kernel uses on pages and page tables,
    including kernel-only attributes. Not all are reachable via attribs_from_word. *)
 datatype vm_attribute = ParityEnabled | PageCacheable | Global | XNever
 type_synonym vm_attributes = "vm_attribute set"
 
-type_synonym arch_raw_vmattrs = word32
+type_synonym arch_raw_vmattrs = machine_word
 
-definition
-  attribs_from_word :: "word32 \<Rightarrow> vm_attributes" where
+definition attribs_from_word :: "machine_word \<Rightarrow> vm_attributes" where
   "attribs_from_word w \<equiv>
-    let V = (if w !!0 then {PageCacheable} else {});
-      V' = (if w!!1 then insert ParityEnabled V else V)
-    in if w!!2 then insert XNever V' else V'"
+     let V = (if w !!0 then {PageCacheable} else {});
+         V' = (if w!!1 then insert ParityEnabled V else V)
+     in if w!!2 then insert XNever V' else V'"
 
-definition
-  attribs_to_word :: "vm_attributes \<Rightarrow> word32" where
+definition attribs_to_word :: "vm_attributes \<Rightarrow> machine_word" where
   "attribs_to_word attribs \<equiv>
-    let V = (if PageCacheable \<in> attribs then 1 else 0);
-      V' = (if ParityEnabled \<in> attribs then V + 2 else V)
-    in if XNever \<in> attribs then V' + 4 else V' "
+     let V = (if PageCacheable \<in> attribs then 1 else 0);
+         V' = (if ParityEnabled \<in> attribs then V + 2 else V)
+     in if XNever \<in> attribs then V' + 4 else V' "
 
-definition
-  validate_vm_attributes :: "word32 \<Rightarrow> vmpage_size \<Rightarrow> word32"  where
+definition validate_vm_attributes :: "machine_word \<Rightarrow> vmpage_size \<Rightarrow> machine_word"  where
   "validate_vm_attributes attr sz \<equiv> case sz of
-    ARM.ARMSmallPage \<Rightarrow> attribs_to_word (attribs_from_word attr - {Global, ParityEnabled})
-  | ARM.ARMLargePage \<Rightarrow> attribs_to_word (attribs_from_word attr - {Global, ParityEnabled})
-  | ARM.ARMSection \<Rightarrow> attribs_to_word (attribs_from_word attr - {Global})
-  | ARM.ARMSuperSection \<Rightarrow> attribs_to_word (attribs_from_word attr - {Global})"
+     ARM.ARMSmallPage \<Rightarrow> attribs_to_word (attribs_from_word attr - {Global, ParityEnabled})
+   | ARM.ARMLargePage \<Rightarrow> attribs_to_word (attribs_from_word attr - {Global, ParityEnabled})
+   | ARM.ARMSection \<Rightarrow> attribs_to_word (attribs_from_word attr - {Global})
+   | ARM.ARMSuperSection \<Rightarrow> attribs_to_word (attribs_from_word attr - {Global})"
 
-definition
-  validate_pt_vm_attributes :: "word32 \<Rightarrow> word32"  where
+definition validate_pt_vm_attributes :: "machine_word \<Rightarrow> machine_word"  where
   "validate_pt_vm_attributes attr \<equiv> attribs_to_word (attribs_from_word attr \<inter> {ParityEnabled})"
 
-definition default_vmattrs :: "word32" where "default_vmattrs \<equiv> 3"
+definition default_vmattrs :: "machine_word" where
+  "default_vmattrs \<equiv> 3"
 
 end
 end
